1. Develop
$$
\begin{align*}
(-3)^4 &= 81 \\
-3^4 &= -81 \\
3^{-4} &= \frac{1}{81} \\
\frac{5^{23}}{5^{21}} = 5^2 &= 25 \\
(\frac{2}{3})^{-2} = \frac{\frac{1}{2^2}}{\frac{1}{3^2}} &= \frac{9}{4} \\
16^{-3/4} = \frac{1}{16^{3/4}} = \frac{1}{2^3} &= \frac{1}{8}
\end{align*}
$$
2. Simplify, without negative exponents
$$
\begin{align*}
\sqrt{200}-\sqrt{32} = 10\sqrt{2}-4\sqrt{2} &= 6\sqrt{2} \\
(3a^3b^3)(4ab^2)^2 &= 48a^5b^7\\
(\frac{3x^{3/2}y^3}{x^2y^{-1/2}})^{-2} = \frac{3^{-2}x^{-3}y^{-6}}{x^{-4}y} &= \frac{x}{9y^7} \\
\end{align*}
$$
3. Expand & Simplify
$$
\begin{align}
3(x+6)+4(2x-5) = 3x+18+8x-20 = 11x-2 \\
(x+3)(4x-5) = 4x^2 -5x + 12x - 15 = 4x^2 + 7x -15 \\
(\sqrt{a}+\sqrt{b})(\sqrt{a}-\sqrt{b}) = a -\sqrt{a}\sqrt{b} + \sqrt{a}\sqrt{b} - b = a - b \\
(2x+3)^2 = 4x^2 + 12x + 9 \\
(x+2)^3 = (x+2)(x^2 + 4x + 4) = x^3 + 4x^2 + 4x + 2x^2 + 8x + 8 = x^3 + 6x^2 + 12x + 8 \\
\end{align}
$$
4. Factor
$$
\begin{align}
4x^2 - 25 = (2x+5)(2x-5) \\

\end{align}
$$
